Extension finished!!!

lean/poly.lean
@@ -1,20 +1,50 @@
 import .lovelib
+import data.set
+open set
 
 @[derive decidable_eq]
 inductive ty : Type
 | TNat : ty
 | TBool : ty
 | TFun : ty → ty → ty
+| TVar : ℕ → ty
+| TForAll : ty → ty
+
+@[derive decidable_eq]
+inductive bi : Type
+| VarBind : ty → bi
+| TarBind : bi -- Tar is short for type variable, to have same length as Var
 
 #print decidable_eq
 #check decidable
 #check has_equiv
+#check option
+
+-- -- type context
+-- inductive ctx : Type
+-- | ctx_nil : ctx
+-- | ctx_snoc (Γ : ctx) (x : bi) : ctx
+
+-- -- operation to lookup the type of a variable in a typing context:
+-- def ctx_lookup_bi (x : bi) : ctx → option bi
+-- | ctx.ctx_nil          := option.none
+-- | (ctx.ctx_snoc Γ y) := if y = x then option.some y else ctx_lookup_bi Γ
+
+-- operation to lookup the type of a variable in a typing context:
+def bi_lookup (i : ℕ) (Γ : list bi) : option ty :=
+match (list.nth Γ i) with
+| none := none
+| some b := match b with
+  | bi.VarBind t := some t
+  | _ := none
+  end
+end
 
 -- define all expressions
 inductive exp : Type
-| EVar (x : string) : exp -- Type of Var(x)
-| ELam (x : string) (A : ty) (e : exp) : exp
-| ERec (f x : string) (A B : ty) (e : exp) : exp -- TFun A → B
+| EVar (i : ℕ) : exp -- Type of Var(x)
+| ELam (A : ty) (e : exp) : exp
+| ERec (A B : ty) (e : exp) : exp -- TFun A → B
 | EApp (e1 e2 : exp) : exp -- Type of e1 (Type of e2)
 | ETrue : exp -- TBool
 | EFalse : exp -- TBool
@@ -24,212 +54,54 @@ inductive exp : Type
 | EPred : exp -- TNat → TNat
 | EIsZero : exp -- TNat → TBool
 
--- type context
-inductive ctx : Type
-| ctx_nil : ctx
-| ctx_snoc (Γ : ctx) (x : string) (A : ty) : ctx
+| ETAbs (e : exp) : exp
+| ETApp (e : exp) (T : ty) : exp
 
--- operation to lookup the type of a variable in a typing context:
-def ctx_lookup (x : string) : ctx → option ty
-| ctx.ctx_nil          := option.none
-| (ctx.ctx_snoc Γ y A) := if y = x then option.some A else ctx_lookup Γ
+def add_bi (ctx : list bi) (b : bi) : list bi := (b::ctx)
 
-inductive typed : ctx → exp → ty → Prop
-| Var_typed (Γ : ctx) (x : string) (A : ty) (p : ctx_lookup x Γ = option.some A) : typed Γ (exp.EVar x) A
-| True_typed {Γ : ctx} : typed Γ exp.ETrue ty.TBool
-| False_typed {Γ : ctx} : typed Γ exp.EFalse ty.TBool
-| If_typed (Γ : ctx) (e1: exp) (e2: exp) (e3: exp) (A: ty) (p1 : typed Γ e1 ty.TBool) (p2: typed Γ e2 A) (p3: typed Γ e3 A) : typed Γ (exp.EIf e1 e2 e3) A
-| Zero_typed {Γ : ctx} : typed Γ exp.Ezero ty.TNat
-| Succ_typed {Γ : ctx} (A : ty) (p : (ty.TFun ty.TNat ty.TNat) = A): typed Γ exp.ESucc A
-| Pred_typed {Γ : ctx} (A : ty) (p : (ty.TFun ty.TNat ty.TNat) = A): typed Γ exp.EPred A
-| IsZero_typed {Γ : ctx} (A : ty) (p : (ty.TFun ty.TNat ty.TBool) = A) : typed Γ exp.EIsZero A
-| Lam_typed (Γ : ctx) (x : string) (e : exp) (aa et A : ty) (p : (ty.TFun aa et) = A) (p2 : typed (ctx.ctx_snoc Γ x aa) e et) : typed Γ (exp.ELam x aa e) A
-| Rec_typed (Γ : ctx) (f: string) (x : string) (aa bb A: ty) (e : exp) (p1 : (ty.TFun aa bb) = A) (p2: typed (ctx.ctx_snoc (ctx.ctx_snoc Γ x aa) f (ty.TFun aa bb)) e bb) : typed Γ (exp.ERec f x aa bb e) A
-| App_typed (Γ : ctx) (e1 e2 : exp) (e2t A : ty) (p1 : typed Γ e2 e2t) (p2 : typed Γ e1 (ty.TFun e2t A)) : typed Γ (exp.EApp e1 e2) A
+def typeShiftAbove : ty → ℕ → ℕ → ty
+| (ty.TVar x) d cc := if x >= cc then ty.TVar (x + d) else ty.TVar(x)
+| (ty.TFun t1 t2) d cc := ty.TFun (typeShiftAbove t1 d cc) (typeShiftAbove t2 d cc)
+| (ty.TForAll t) d cc := ty.TForAll (typeShiftAbove t d (cc + 1))
+| tyT _ _ := tyT
 
--- Exercise 2
-constants (Γ : ctx)
-lemma test_id_nat : typed Γ (exp.ELam "x" ty.TNat (exp.EVar "x")) (ty.TFun ty.TNat ty.TNat) :=
-  begin
-    apply typed.Lam_typed,
-    refl,
-    apply typed.Var_typed,
-    simp [ctx_lookup],
-  end
+def typeShiftBelow : ty → ℕ → ℕ → ty
+| (ty.TVar x) d cc := if x >= cc then ty.TVar (x - d) else ty.TVar(x)
+| (ty.TFun t1 t2) d cc := ty.TFun (typeShiftAbove t1 d cc) (typeShiftAbove t2 d cc)
+| (ty.TForAll t) d cc := ty.TForAll (typeShiftAbove t d (cc + 1))
+| tyT _ _ := tyT
 
-lemma test_isZero : typed Γ (exp.ELam "x" ty.TNat exp.EIsZero) (ty.TFun ty.TNat (ty.TFun ty.TNat ty.TBool)) :=
-  begin
-    apply typed.Lam_typed,
-    refl,
-    apply typed.IsZero_typed,
-    refl,
-  end
+def tsa (d : ℕ) (tyT : ty) : ty := typeShiftAbove tyT d 0
+def tsb (d : ℕ) (tyT : ty) : ty := typeShiftBelow tyT d 0
 
-lemma test_everything : typed Γ
-  (exp.ERec "f" "x" ty.TNat ty.TNat (exp.EIf (exp.EApp exp.EIsZero (exp.EVar "x")) (exp.Ezero) (exp.EApp exp.ESucc (exp.EApp exp.ESucc (exp.EApp (exp.EVar "f") (exp.EApp exp.EPred (exp.EVar "x"))))))) (ty.TFun ty.TNat ty.TNat) :=
-  begin
-    apply typed.Rec_typed,
-    refl,
-    apply typed.If_typed,
-      apply typed.App_typed,
-      apply typed.Var_typed,
-      simp [ctx_lookup],
-      refl,
-    apply typed.IsZero_typed,
-    refl,
-    apply typed.Zero_typed,
-    apply typed.App_typed,
-    apply typed.App_typed,
-    apply typed.App_typed,
-    apply typed.App_typed,
-    apply typed.Var_typed,
-    simp [ctx_lookup],
-    refl,
-    apply typed.Pred_typed,
-    refl,
-    apply typed.Var_typed,
-    simp [ctx_lookup],
-    apply typed.Succ_typed,
-    refl,
-    apply typed.Succ_typed,
-    refl,
-  end
+def typeSubst : ty → ty → ℕ → ty
+| (ty.TVar i) tyS c := if i = c then tsa c tyS else (ty.TVar i)
+| (ty.TFun t1 t2) tyS c := ty.TFun (typeSubst t1 tyS c) (typeSubst t2 tyS c)
+| (ty.TForAll t) tyS c := ty.TForAll(typeSubst t tyS (c + 1))
+| tyT _ _ := tyT
 
--- def f(x : Nat) : Nat → Bool:
---   return lambda y : Nat:
---     if x == 0:
---       if y == 0:
---         return true
---       else:
---         return false
---     else:
---       if y == 0:
---         return false
---       else:
---         return (f(x - 1))(y - 1)
-lemma test_check_equal : typed Γ
-(
-  exp.ERec "f" "x" ty.TNat (ty.TFun ty.TNat ty.TBool)
-  (
-    exp.ELam "y" ty.TNat
-    (
-      exp.EIf (exp.EApp exp.EIsZero (exp.EVar "x"))
-      (
-        exp.EIf (exp.EApp exp.EIsZero (exp.EVar "y"))
-          exp.ETrue
-          exp.EFalse
-      )
-      (
-        exp.EIf (exp.EApp exp.EIsZero (exp.EVar "y"))
-          exp.EFalse
-          (
-            exp.EApp
-            (exp.EApp (exp.EVar "f") (exp.EApp exp.EPred (exp.EVar "x")))
-            (exp.EApp exp.EPred (exp.EVar "y"))
-          )
-      )
-    )
-  )
-)
-(ty.TFun ty.TNat (ty.TFun ty.TNat ty.TBool)) :=
-begin
-  apply typed.Rec_typed,
-  {
-    refl,
-  },
-  {
-    apply typed.Lam_typed,
-    {
-      refl,
-    },
-    {
-      apply typed.If_typed,
-      {
-        apply typed.App_typed,
-        {
-          apply typed.Var_typed,
-            refl,
-        },
-        {
-          apply typed.IsZero_typed,
-            refl,
-        },
-      },
-      {
-        apply typed.If_typed,
-        {
-          apply typed.App_typed,
-          {
-            apply typed.Var_typed,
-              refl,
-          },
-          {
-            apply typed.IsZero_typed,
-              refl,
-          },
-        },
-        {
-          apply typed.True_typed,
-        },
-        {
-          apply typed.False_typed,
-        },
-      },
-      {
-        apply typed.If_typed,
-        {
-          apply typed.App_typed,
-          {
-            apply typed.Var_typed,
-              refl,
-          },
-          {
-            apply typed.IsZero_typed,
-              refl,
-          },
-        },
-        {
-          apply typed.False_typed,
-        },
-        {
-          apply typed.App_typed,
-          {
-            apply typed.App_typed,
-            {
-              apply typed.Var_typed,
-              refl,
-            },
-            {
-              apply typed.Pred_typed,
-                refl,
-            },
-          },
-          {
-            apply typed.App_typed,
-            {
-              apply typed.App_typed,
-              {
-                apply typed.Var_typed,
-                refl,
-              },
-              {
-                apply typed.Pred_typed,
-                  refl,
-              },
-            },
-            {
-              apply typed.Var_typed,
-                refl,
-            },
-          },
-        }
-      },
-    },
-  },
-end
+def typeSubstTop (tyS tyT : ty): ty :=
+  tsb 1 (typeSubst tyT (tsa 1 tyS) 0)
 
-def type_infer : ctx → exp → option ty
-| Γ (exp.EVar x)           := ctx_lookup x Γ
+
+inductive typed : list bi → exp → ty → Prop
+| Var_typed (Γ : list bi) (x : ℕ) (A : ty) (p : bi_lookup x Γ = option.some A) : typed Γ (exp.EVar x) A
+| True_typed {Γ : list bi} : typed Γ exp.ETrue ty.TBool
+| False_typed {Γ : list bi} : typed Γ exp.EFalse ty.TBool
+| If_typed (Γ : list bi) (e1: exp) (e2: exp) (e3: exp) (A: ty) (p1 : typed Γ e1 ty.TBool) (p2: typed Γ e2 A) (p3: typed Γ e3 A) : typed Γ (exp.EIf e1 e2 e3) A
+| Zero_typed {Γ : list bi} : typed Γ exp.Ezero ty.TNat
+| Succ_typed {Γ : list bi} (A : ty) (p : (ty.TFun ty.TNat ty.TNat) = A): typed Γ exp.ESucc A
+| Pred_typed {Γ : list bi} (A : ty) (p : (ty.TFun ty.TNat ty.TNat) = A): typed Γ exp.EPred A
+| IsZero_typed {Γ : list bi} (A : ty) (p : (ty.TFun ty.TNat ty.TBool) = A) : typed Γ exp.EIsZero A
+| Lam_typed (Γ : list bi) (e : exp) (aa et A : ty) (p : (ty.TFun aa et) = A) (p2 : typed (add_bi Γ (bi.VarBind aa)) e et) : typed Γ (exp.ELam aa e) A
+| Rec_typed (Γ : list bi) (aa bb A: ty) (e : exp) (p1 : (ty.TFun aa bb) = A) (p2: typed (add_bi (add_bi Γ (bi.VarBind aa)) (bi.VarBind (ty.TFun aa bb))) e bb) : typed Γ (exp.ERec aa bb e) A
+| App_typed (Γ : list bi) (e1 e2 : exp) (e2t A : ty) (p1 : typed Γ e2 e2t) (p2 : typed Γ e1 (ty.TFun e2t A)) : typed Γ (exp.EApp e1 e2) A
+
+| TAbs_typed {Γ : list bi} (e : exp) (A T: ty) (p1 : typed (add_bi Γ bi.TarBind) e A) (p2 : T = ty.TForAll A): typed Γ (exp.ETAbs e) T
+| TApp_typed {Γ : list bi} (tt1 : exp) (TT2 A : ty) {TT12 : ty} (p1 : typed Γ tt1 (ty.TForAll TT12)) (p2 : typeSubstTop TT2 TT12 = A) : typed Γ (exp.ETApp tt1 TT2) A -- TODO: here should not be T,
+
+def type_infer : list bi → exp → option ty
+| Γ (exp.EVar x)           := bi_lookup x Γ
 | Γ exp.ETrue              := some ty.TBool
 | Γ exp.EFalse             := some ty.TBool
 | Γ (exp.EIf e1 e2 e3)     :=
@@ -245,13 +117,13 @@ def type_infer : ctx → exp → option ty
 | Γ exp.ESucc             := some (ty.TFun ty.TNat ty.TNat)
 | Γ exp.EPred             := some (ty.TFun ty.TNat ty.TNat)
 | Γ exp.EIsZero           := some (ty.TFun ty.TNat ty.TBool)
-| Γ (exp.ELam x A e)      :=
-  match type_infer (ctx.ctx_snoc Γ x A) e with
+| Γ (exp.ELam A e)      :=
+  match type_infer (add_bi Γ (bi.VarBind A)) e with
   | some B  := some (ty.TFun A B)
   | none    := none
   end
-| Γ (exp.ERec f x A B e)  :=
-  match type_infer (ctx.ctx_snoc (ctx.ctx_snoc Γ x A) f (ty.TFun A B)) e with
+| Γ (exp.ERec A B e)  :=
+  match type_infer (add_bi (add_bi Γ (bi.VarBind A)) (bi.VarBind (ty.TFun A B))) e with
   | some C := if B = C then some (ty.TFun A B) else none
   | _ := none
   end
@@ -260,8 +132,21 @@ def type_infer : ctx → exp → option ty
   | some (ty.TFun A B), some C := if A = C then some B else none
     | _, _                 := none
   end
+| Γ (exp.ETAbs e) :=
+  match type_infer (add_bi Γ (bi.TarBind)) e with
+  | some C := some (ty.TForAll C)
+  | _ := none
+  end
+| Γ (exp.ETApp e t) :=
+  match type_infer Γ e with
+  | some ty1 := match ty1 with
+    | ty.TForAll ttt := some (typeSubstTop t ttt)
+    | _ := none
+    end
+  | _ := none
+  end
 
-lemma type_infer_complete (Γ : ctx) (e : exp) (A : ty) : typed Γ e A → type_infer Γ e = option.some A :=
+lemma type_infer_complete (Γ : list bi) (e : exp) (A : ty) : typed Γ e A → type_infer Γ e = option.some A :=
 begin
   intro h,
   induction h,
@@ -282,24 +167,25 @@ begin
       exact h_p1,
     },
     simp [type_infer, h_p1, h_p2, h_ih_p1, h_ih_p2],
+    -- These tow line are extended for ETAbs and ETApp
+    simp [type_infer, h_p1, h_p2, h_ih],
+    simp [type_infer, h_p1, h_p2, h_ih, typeSubstTop],
+    -- simp [typeSubstTop, typeSubst, tsb, tsa, typeShiftBelow, typeShiftAbove] at h_p3,
+    finish,
 end
 
--- Acknowledge
--- https://www.cs.cornell.edu/courses/cs4160/2019sp/terse/plf/Typechecking.html
--- Although I read the above link, it is still a tough proof for me
--- I guess I should use a lot of finishes to shrink the proof a lot and a lot
 lemma type_infer_sound: ∀Γ e A, type_infer Γ e = option.some A → typed Γ e A :=
 begin
   intros Γ e,
   revert Γ,
   induction' e;
-  intros Γ T h;
+  intros Γ TT h;
   cases' h,
 
   {
     -- case Var
     simp [type_infer] at cases_eq,
-    destruct (ctx_lookup x Γ),
+    destruct (bi_lookup i Γ),
     intro htt,
     apply typed.Var_typed,
       exact cases_eq,
@@ -310,9 +196,9 @@ begin
   {
     -- case Lam
     simp [type_infer] at cases_eq,
-    generalize htt : Γ.ctx_snoc x A = GG,
+    generalize htt : add_bi Γ (bi.VarBind A) = GG,
     generalize hto : type_infer GG e = TOO,
-    have httr : GG = Γ.ctx_snoc x A, from
+    have httr : GG = add_bi Γ (bi.VarBind A), from
       begin
         apply eq.symm,
         exact htt,
@@ -339,16 +225,16 @@ begin
   {
     -- case Rec
     simp [type_infer] at cases_eq,
-    generalize htt : Γ.ctx_snoc x A = GG,
-    generalize httt : GG.ctx_snoc f (A.TFun B) = GGG,
+    generalize htt : add_bi Γ (bi.VarBind A) = GG,
+    generalize httt : add_bi GG (bi.VarBind (A.TFun B)) = GGG,
     generalize hto : type_infer GGG e = TOOO,
-    have httr : GG = Γ.ctx_snoc x A, from
+    have httr : GG = add_bi Γ (bi.VarBind A), from
       begin
         apply eq.symm,
         exact htt,
       end,
     rw [httr] at httt,
-    have htttr : GGG = (Γ.ctx_snoc x A).ctx_snoc f (A.TFun B), from
+    have htttr : GGG = add_bi (add_bi Γ (bi.VarBind A)) (bi.VarBind(A.TFun B)), from
       begin
         apply eq.symm,
         exact httt,
@@ -413,6 +299,12 @@ begin
           simp [type_infer] at cases_eq,
           exact cases_eq,
 
+          simp [type_infer] at cases_eq,
+          exact cases_eq,
+
+          simp [type_infer] at cases_eq,
+          exact cases_eq,
+
         apply typed.App_typed,
           swap 3,
           exact val_1,
@@ -447,6 +339,10 @@ begin
             simp [option.iget] at cases_eq,
             simp *,
             assumption,
+
+            -- Is this magic?
+            finish,
+            finish,
   },
   {
     -- case True
@@ -553,6 +449,9 @@ begin
         simp [type_infer] at cases_eq,
         by_contra,
         exact cases_eq,
+
+        finish,
+        finish,
   },
   {
     -- case Zero
@@ -569,5 +468,59 @@ begin
   {
     -- case IsZero
     simp [typed.IsZero_typed],
+  },
+  {
+    -- case Type Abs
+    simp [type_infer] at cases_eq,
+    generalize htt : add_bi Γ bi.TarBind = GG,
+    generalize hto : type_infer GG e = TOO,
+    have httr : GG = add_bi Γ bi.TarBind, from
+      begin
+        apply eq.symm,
+        exact htt,
+      end,
+    rw [httr] at hto,
+    rw [hto] at cases_eq,
+    cases' TOO,
+      by_contra,
+      simp [type_infer] at cases_eq,
+      exact cases_eq,
+
+      apply typed.TAbs_typed,
+        -- Need to fix the type variable first
+        swap 3,
+        exact val,
+
+        simp [type_infer] at cases_eq,
+        apply ih,
+        exact hto,
+
+        simp [type_infer] at cases_eq,
+        simp [cases_eq],
+  },
+  {
+    -- case TApp
+    simp [type_infer] at cases_eq,
+    generalize hto : type_infer Γ e = TO,
+    cases' TO,
+      by_contra,
+      finish,
+
+      rw [hto] at cases_eq,
+      simp [type_infer, typeSubstTop] at cases_eq,
+      cases' val,
+        finish,
+        finish,
+        finish,
+        finish,
+        apply typed.TApp_typed,
+        swap 3,
+          exact val,
+
+          apply ih,
+          exact hto,
+
+          simp [type_infer] at cases_eq,
+          exact cases_eq,
   },
 end
